apa.v
@@ -12,11 +12,15 @@ Definition apa_ident_mp (num_cpus: nat) (hp: sched_job_hp_relation) (mapped: job
                     (alpha: affinity) (sched: schedule) :=
   (* The mapping has a finite number of cpus: [1, num_cpus) *)
   << apa_cpus_nonzero: num_cpus > 0 >> /\
-  << apa_num_cpus: forall j cpu t, mapped j cpu t <-> cpu < num_cpus >> /\
+  << apa_num_cpus: forall j cpu t, mapped j cpu t -> cpu < num_cpus >> /\
 
   (* Job is scheduled iff it is mapped to a processor*)
-  << apa_mapping: forall j cpu t, scheduled sched j t <-> mapped j cpu t >> /\
+  << apa_mapping: forall j t, scheduled sched j t <-> exists cpu, mapped j cpu t >> /\
 
+  (* Non-parallelism restrictions (mapping must be an injective function) *)
+  << mp_mapping_fun: forall j cpu cpu' t, mapped j cpu t /\ mapped j cpu' t -> cpu = cpu' >> /\
+  << mp_mapping_inj: forall j j' cpu t, mapped j cpu t /\ mapped j' cpu t -> j = j'>> /\
+                                                                  
   (* A job receives at most 1 unit of service *)
   << apa_max_service: forall j t, service_at sched j t <= 1 >> /\
 
@@ -43,35 +47,27 @@ Lemma exists_apa_platform_that_is_global :
             service sched j t = service sched' j t.
 Proof.
  ins; exists (fun j cpu => True).
- unfold apa_ident_mp; ins; des.
+ ins; des.
  induction t.
    (* Base case *)
    (* Inductive Step *)
-
-
 Admitted.
 
-(* Definitions for APA affinity restoration *)
+(* Definitions for APA affinity restoration -- IGNORE *)
 
 (* Per-task affinities *)
 Definition task_affinity (alpha: affinity) :=
    forall (tsk: sporadic_task) (j1 j2: job),
-       job_of j1 = Some tsk /\ job_of j2 = Some tsk -> alpha j1 = alpha j2.
+       job_task j1 = tsk /\ job_task j2 = tsk -> alpha j1 = alpha j2.
 
-Definition inter : set nat -> set nat -> set nat := set_inter eq_nat_dec.
-
-Definition restrict (tsk_i: sporadic_task) (ts: taskset) (alpha: affinity) (alpha': affinity) :=
-  << ALPHA: task_affinity alpha >> /\
-  << ALPHA': task_affinity alpha' >> /\
-  forall tsk j j_i (INtsk: In tsk ts) (INtsk_i: In tsk_i ts) (JOBj: job_of j = Some tsk)
-         (JOBj_i: job_of j_i = Some tsk_i), alpha' j = inter (alpha j) (alpha j_i).
+Definition restrict (tsk_i: sporadic_task) (ts: taskset) (alpha1 alpha2 alpha': affinity) := True.
 
 (* Service invariant from APA paper *)
 Lemma APA_service_invariant :
-  forall num_cpus sched hp cpumap ts alpha alpha' tsk_i j t
+  forall num_cpus sched hp cpumap ts alpha alpha' (tsk_i: sporadic_task) j t
          (APA: apa_ident_mp num_cpus hp cpumap alpha sched) (INtsk_i: In tsk_i ts)
          (ALPHAtsk: task_affinity alpha) (ALPHA'tsk: task_affinity alpha')
-         (RESTR: restrict tsk_i ts alpha alpha'),
+         (*(RESTR: ...)*),
     exists sched' cpumap',
        << APA': apa_ident_mp num_cpus hp cpumap' alpha' sched' >> /\
        << SERV: service sched j t >= service sched' j t >>.
