liulayland.v
@@ -3,11 +3,10 @@ Require Import List Arith Sorting Vbase job task schedule identmp priority helpe
 Section LiuLayland.
 Variable ts: taskset.
 Variable sched: schedule.
-Variable hp: higher_priority.
-Variable cpumap: processor_list.
+Variable hp: sched_job_hp_relation.
+Variable cpumap: job_mapping.
 
-Definition task_hp := fp_higher_priority RM. (* Rate-monotonic priority *)
-Hypothesis RM_priority : fixed_priority hp task_hp. (* Link job priority with task priority *)
+Hypothesis RM_priority : convert_fp_jldp RM hp.
 
 Definition uniprocessor := ident_mp 1 hp cpumap. (* Uniprocessor system *)
 Hypothesis platform : uniprocessor sched.
@@ -17,77 +16,38 @@ Hypothesis periodic_tasks: periodic_task_model ts sched.
 Hypothesis implicit_deadlines: implicit_deadline_model ts.
 
 Hypothesis ts_non_empty: ts <> nil.
-Hypothesis ts_sorted_by_prio: StronglySorted task_hp ts. 
+Hypothesis ts_sorted_by_prio: StronglySorted RM ts. 
 
-Hypothesis job_cost_wcet: forall j t tsk (JOBj: job_of j = Some tsk) (ARRj: arrives_at sched j t), job_cost j = task_cost tsk.
-
-(* Simpler scheduling invariant for uniprocessor (eliminates cpu mapping) *)
-Lemma uni_simpler_invariant :
-  forall jlow t, 
-    backlogged sched jlow t <-> exists jhigh, hp sched t jhigh jlow /\ scheduled sched jhigh t.
-Proof.
-  rename platform into PLAT.
-  unfold uniprocessor, ident_mp in *; split; intro BL; des; specialize (mp_invariant jlow t).
-  {
-    destruct mp_invariant as [mp_invariant _].
-    apply mp_invariant with (cpu := 0) in BL; [| by eauto]; des.
-    exists jhigh; split; [by eauto|].
-    rewrite <- mp_mapping.
-    eauto using element_in_list.
-  }
-  {
-    destruct mp_invariant as [_ mp_invariant].
-    apply mp_invariant; ins.
-    exists jhigh; split; [by eauto|].
-    apply In_singleton_list; eauto.
-      by rewrite mp_mapping.
-  }
-Qed.
+Hypothesis job_cost_wcet: forall j t tsk (JOBj: job_task j = tsk) (ARRj: arrives_at sched j t), job_cost j = task_cost tsk.
 
 Lemma periodic_arrival_k_times : 
-  forall j tsk (JOBj: job_of j = Some tsk) t (ARRj: arrives_at sched j t) k,
-    exists j', << JOBj': job_of j' = Some tsk >> /\
+  forall j tsk (JOBj: job_task j = tsk) t (ARRj: arrives_at sched j t) k,
+    exists j', << JOBj': job_task j' = tsk >> /\
                << ARRj': arrives_at sched j' (t + k*(task_period tsk)) >>.
 Proof.
-  revert periodic_tasks; unfold periodic_task_model; intros PER; ins.
-  specialize (PER arr_seq_from_ts).
+  revert periodic_tasks; unfold periodic_task_model; intros PER; ins; des.
   induction k; simpl; des.
     by rewrite <- plus_n_O; eauto.
     {
-      apply PER with (t := t + k*(task_period tsk)) in JOBj'; eauto; des; subst.
-      exists j'0; split; eauto.
-      assert (COMM : t + k * task_period tsk + task_period tsk =
-                     t + (task_period tsk + k * task_period tsk)); [by omega |].
+      apply PER0 in ARRj'; des; subst; rewrite JOBj' in *.
+      exists j'0; split; eauto using eq_trans.
+      assert (COMM : t + k * task_period (job_task j) + task_period (job_task j) =
+                     t + (task_period (job_task j) + k * task_period (job_task j))); [by omega |].
       rewrite <- COMM; trivial.
     }
 Qed.
 
-Lemma sync_release_is_critical_instant :
+(*Lemma sync_release_is_critical_instant :
   forall t tsk_i (INi: In tsk_i ts) (SYNC: sync_release ts sched t),
     critical_instant uniprocessor tsk_i ts sched t.
 Proof.
-  revert ts_sorted_by_prio; intro SORTED.
-  unfold sync_release, critical_instant; ins.
-  assert (ARRi := SYNC tsk_i INi); des.
-  exists j; repeat (split; eauto); ins.
-  unfold task_response_time_ub. intros _ sched' j' t' r'; ins.
-
-  inversion SORTED; subst.
-    by intuition.
-    
-
+Admitted.
 
 Lemma hp_task_no_interference :
     forall (tsk_i: sporadic_task),
         Forall (task_hp tsk_i) ts ->
             task_response_time tsk_i (tsk_i :: ts) (task_cost tsk_i).
 Proof.
-    intros tsk_i tsk_i_hp.
-    unfold task_response_time.
-    split. simpl. apply or_introl. trivial.
-    generalize sched.
-    clear periodic_tasks arr_seq_from_ts uniprocessor sched.
-    intros sched uniprocessor arr_seq_from_ts periodic_tasks.
-
+Admitted.*)
 
 End LiuLayland.
